Graph.v
@@ -83,6 +83,16 @@ Module Type Graph (O: UsualOrderedType)(S: FSetInterface.Sfun O).
   Parameter set_of_graph_1: forall g v,
     contains_vertex g v = true <-> S.In v (set_of_graph g).
 
+  (*TODO: see if better way to define in interface*)
+  (*A topological ordering is one where there are no edges going backward in the list and every vertex in the 
+  graph is in the list*)
+  Parameter topological_sort: list vertex -> graph ->  Prop.
+
+  Parameter topological_sort_def: forall l g,
+    topological_sort l g <-> 
+  (forall v, contains_vertex g v = true <-> In v l) /\ NoDup l /\
+  (forall l1 l2 l3 u v, l = l1 ++ u :: l2 ++ v :: l3 -> contains_edge g v u = false).
+
 
 End Graph.
 
